Simple solver.

Leanr/AlgebraicConstraint.lean
@@ -3,7 +3,7 @@ import Leanr.Expression
 structure AlgebraicConstraint (p : ℕ) where
   expression : Expression p
 
-def AlgebraicConstraint.is_satisfied {p : ℕ}
+def AlgebraicConstraint.is_satisfied_by {p : ℕ}
   (c : AlgebraicConstraint p)
   (env : String → ZMod p) : Prop :=
   c.expression.eval env = 0
@@ -13,3 +13,9 @@ def AlgebraicConstraint.substitute {p : ℕ}
   (x : String)
   (v : ZMod p) : AlgebraicConstraint p :=
   { expression := c.expression.substitute x v }
+
+def AlgebraicConstraint.trivial {p : ℕ}
+  (c : AlgebraicConstraint p) : Prop :=
+  match c.expression with
+  | .const c => if c.val = 0 then true else false
+  | _ => false
